.

theories/Prelude/PreludeMath.v
@@ -1,3 +1,4 @@
+Require Import Coq.Arith.PeanoNat.
 Require Import Coq.Classes.RelationClasses.
 Require Import Coq.Lists.List.
 Require Import Coq.Program.Basics.
@@ -5,6 +6,7 @@ Require Import Coq.Relations.Relation_Definitions.
 Require Import Coq.Relations.Relation_Operators.
 Require Import Coq.Setoids.Setoid.
 Require Import DschingisKhan.Prelude.PreludeInit.
+Require Import DschingisKhan.Prelude.PreludeUtil.
 
 Module MathPrelude.
 
@@ -13,33 +15,40 @@ Module MathPrelude.
   (** "0. Utilities" *)
 
   Class isUnaryOperationCompatibleWithSetoid {dom : Hask.t} {cod : Hask.t} {dom_isSetoid : isSetoid dom} {cod_isSetoid : isSetoid cod} (f : dom -> cod) : Prop :=
-    unary_operation_preserves_eqProp (lhs : dom) (rhs : dom) (H_EQ : lhs == rhs) : f lhs == f rhs
+    unary_operation_preserves_eqProp (lhs : dom) (rhs : dom)
+    (H_EQ : lhs == rhs)
+    : f lhs == f rhs
   .
 
   Class isBinaryOperationCompatibleWithSetoid {dom1 : Hask.t} {dom2 : Hask.t} {cod : Hask.t} {dom1_isSetoid : isSetoid dom1} {dom2_isSetoid : isSetoid dom2} {cod_isSetoid : isSetoid cod} (f : dom1 -> dom2 -> cod) : Prop :=
-    binary_operation_preserves_eqProp (lhs1 : dom1) (rhs1 : dom1) (lhs2 : dom2) (rhs2 : dom2) (H_EQ1 : lhs1 == rhs1) (H_EQ2 : lhs2 == rhs2) : f lhs1 lhs2 == f rhs1 rhs2
+    binary_operation_preserves_eqProp (lhs1 : dom1) (rhs1 : dom1) (lhs2 : dom2) (rhs2 : dom2)
+    (H_EQ1 : lhs1 == rhs1)
+    (H_EQ2 : lhs2 == rhs2)
+    : f lhs1 lhs2 == f rhs1 rhs2
   .
 
-  Global Add Parametric Morphism {dom : Hask.t} {cod : Hask.t} {dom_isSetoid : isSetoid dom} {cod_isSetoid : isSetoid cod} (f : dom -> cod) {f_isCompatible : isUnaryOperationCompatibleWithSetoid f} :
+  Global Add Parametric Morphism {dom : Hask.t} {cod : Hask.t} {dom_isSetoid : isSetoid dom} {cod_isSetoid : isSetoid cod} (f : dom -> cod) {isCompatibleWith_eqProp : isUnaryOperationCompatibleWithSetoid f} :
     f with signature (eqProp ==> eqProp)
     as unary_operation_lifts_eqProp.
-  Proof. ii; apply f_isCompatible; eauto. Qed.
+  Proof. intros x1 x2 H_x_eq; exact (isCompatibleWith_eqProp x1 x2 H_x_eq). Defined.
 
-  Global Add Parametric Morphism {dom1 : Hask.t} {dom2 : Hask.t} {cod : Hask.t} {dom1_isSetoid : isSetoid dom1} {dom2_isSetoid : isSetoid dom2} {cod_isSetoid : isSetoid cod} (f : dom1 -> dom2 -> cod) {f_isCompatible : isBinaryOperationCompatibleWithSetoid f} :
+  Global Add Parametric Morphism {dom1 : Hask.t} {dom2 : Hask.t} {cod : Hask.t} {dom1_isSetoid : isSetoid dom1} {dom2_isSetoid : isSetoid dom2} {cod_isSetoid : isSetoid cod} (f : dom1 -> dom2 -> cod) {isCompatibleWith_eqProp : isBinaryOperationCompatibleWithSetoid f} :
     f with signature (eqProp ==> eqProp ==> eqProp)
     as binary_operation_lifts_eqProp.
-  Proof. ii; apply f_isCompatible; eauto. Qed.
+  Proof. intros x1 x2 H_x_eq y1 y2 H_y_eq; exact (isCompatibleWith_eqProp x1 x2 y1 y2 H_x_eq H_y_eq). Defined.
 
   Section STATEMENTS_FOR_OPERATION_PROPERTIES.
 
   Context {A : Hask.t} {requiresSetoid : isSetoid A}.
 
   Class isAssociativeBinaryOperation (bin_op : A -> A -> A) : Prop :=
-    bin_op_assoc (x : A) (y : A) (z : A) : bin_op x (bin_op y z) == bin_op (bin_op x y) z
+    bin_op_assoc (x : A) (y : A) (z : A)
+    : bin_op x (bin_op y z) == bin_op (bin_op x y) z
   .
 
   Class isCommutativeBinaryOperation (bin_op : A -> A -> A) : Prop :=
-    bin_op_comm (x : A) (y : A) : bin_op x y == bin_op y x
+    bin_op_comm (x : A) (y : A)
+    : bin_op x y == bin_op y x
   .
 
   Class isIdempotentBinaryOperation (bin_op : A -> A -> A) : Prop :=
@@ -47,26 +56,34 @@ Module MathPrelude.
   .
 
   Class isDistributiveOver (bin_op1 : A -> A -> A) (bin_op2 : A -> A -> A) : Prop :=
-    { left_distr (x : A) (y : A) (z : A) : bin_op1 x (bin_op2 y z) == bin_op2 (bin_op1 x y) (bin_op1 x z)
-    ; right_distr (x : A) (y : A) (z : A) : bin_op1 (bin_op2 y z) x == bin_op2 (bin_op1 y x) (bin_op1 z x)
+    { left_distr (x : A) (y : A) (z : A)
+      : bin_op1 x (bin_op2 y z) == bin_op2 (bin_op1 x y) (bin_op1 x z)
+    ; right_distr (x : A) (y : A) (z : A)
+      : bin_op1 (bin_op2 y z) x == bin_op2 (bin_op1 y x) (bin_op1 z x)
     }
   .
 
   Class isIdentity (e : A) (bin_op : A -> A -> A) : Prop :=
-    { left_id (x : A) : bin_op e x == x
-    ; right_id (x : A) : bin_op x e == x
+    { left_id (x : A)
+      : bin_op e x == x
+    ; right_id (x : A)
+      : bin_op x e == x
     }
   .
 
   Class isInverseOperation (inv : A -> A) (bin_op : A -> A -> A) : Prop :=
-    { left_inv (x : A) : bin_op (inv x) x == x
-    ; right_inv (x : A) : bin_op x (inv x) == x
+    { left_inv (x : A)
+      : bin_op (inv x) x == x
+    ; right_inv (x : A)
+      : bin_op x (inv x) == x
     }
   .
 
   Class linkedByAbsorptionLaw (bin_op1 : A -> A -> A) (bin_op2 : A -> A -> A) : Prop :=
-    { abosortion_left (x : A) (y : A) : bin_op1 x (bin_op2 x y) == x
-    ; abosortion_right (x : A) (y : A) : bin_op2 x (bin_op1 x y) == x
+    { abosortion_left (x : A) (y : A)
+      : bin_op1 x (bin_op2 x y) == x
+    ; abosortion_right (x : A) (y : A)
+      : bin_op2 x (bin_op1 x y) == x
     }
   .
 
@@ -78,7 +95,8 @@ Module MathPrelude.
 
   Class isCountable (A : Hask.t) : Type :=
     { enum (n : nat) : A
-    ; enumeratable (x : A) : exists n : nat, enum n = x
+    ; enumeratable (x : A)
+      : exists n : nat, enum n = x
     }
   .
 
@@ -93,7 +111,8 @@ Module MathPrelude.
   .
 
   Class isCoLa (D : Hask.t) {requiresPoset : isPoset D} : Type :=
-    CoLa_isCompleteLattice (X : ensemble D) : {sup_X : D | isSupremumOf sup_X X}
+    CoLa_isCompleteLattice (X : ensemble D)
+    : {sup_X : D | isSupremumOf sup_X X}
   .
 
   Definition isDirectedSubset {D : Hask.t} {requiresPoset : isPoset D} (X : ensemble D) : Prop :=
@@ -104,7 +123,9 @@ Module MathPrelude.
   .
 
   Class isCPO (D : Hask.t) {requiresPoset : isPoset D} : Type :=
-    CPO_isCompletePartialOrder (X : ensemble D) (X_isDirected : isDirectedSubset X) : {sup_X : D | isSupremumOf sup_X X}
+    CPO_isCompletePartialOrder (X : ensemble D)
+    (X_isDirected : isDirectedSubset X)
+    : {sup_X : D | isSupremumOf sup_X X}
   .
 
   (** "2. Topology" *)
@@ -134,30 +155,101 @@ Module MathPrelude.
 
   (** "3. Semigroup, Monoid and Group" *)
 
+  Section AXIOMS_OF_GROUP.
+
+  Variable G : Hask.t.
+
+  Variable requiresSetoid : isSetoid G.
+
+  Class LawsOfSemigroup (add : G -> G -> G) : Prop :=
+    { add_lifts_eqProp :> isBinaryOperationCompatibleWithSetoid add
+    ; add_assoc :> isAssociativeBinaryOperation add
+    }
+  .
+
+  Class LawsOfMonoid (add : G -> G -> G) (zero : G) : Prop :=
+    { Monoid_requiresSemigroup :> LawsOfSemigroup add
+    ; zero_id_add :> zero `isIdentityOf` add
+    }
+  .
+
+  Class LawsOfGroup (add : G -> G -> G) (zero : G) (neg : G -> G) : Prop :=
+    { Group_requiresMonoid :> LawsOfMonoid add zero
+    ; neg_inv_add :> neg `isInverseOpFor` add
+    }
+  .
+
+  End AXIOMS_OF_GROUP.
+
+  Global Arguments LawsOfSemigroup (G) {requiresSetoid}.
+  Global Arguments LawsOfMonoid (G) {requiresSetoid}.
+  Global Arguments LawsOfGroup (G) {requiresSetoid}.
+
+  Class Semigroup_sig (S : Hask.t) : Type :=
+    { add : S -> S -> S
+    }
+  .
+
   Class isSemigroup (S : Hask.t) {requiresSetoid : isSetoid S} : Type :=
-    { plu : S -> S -> S
-    ; plu_lifts_eqProp :> isBinaryOperationCompatibleWithSetoid plu
-    ; plu_assoc :> isAssociativeBinaryOperation plu
+    { Semigroup_methods :> Semigroup_sig S
+    ; obeysLawsOfSemigroup :> LawsOfSemigroup S add
+    }
+  .
+
+  Class Monoid_sig (M : Hask.t) : Type :=
+    { zero : M
+    ; Monoid_has_Semigroup_methods :> Semigroup_sig M
     }
   .
 
   Class isMonoid (M : Hask.t) {requiresSetoid : isSetoid M} : Type :=
-    { zer : M
-    ; Monoid_requiresSemigroup :> isSemigroup M
-    ; zer_id_plu :> zer `isIdentityOf` plu
+    { Monoid_methods :> Monoid_sig M
+    ; obeysLawsOfMonoid :> LawsOfMonoid M add zero
+    }
+  .
+
+  Class Group_sig (G : Hask.t) : Type :=
+    { neg : G -> G
+    ; Group_has_Monoid_methods :> Monoid_sig G
     }
   .
 
   Class isGroup (G : Hask.t) {requiresSetoid : isSetoid G} : Type :=
-    { neg : G -> G
-    ; Group_requiresMonoid :> isMonoid G
-    ; neg_inv_plu :> neg `isInverseOpFor` plu
+    { Group_methods :> Group_sig G
+    ; obeysLawsOfGroup :> LawsOfGroup G add zero neg
     }
   .
 
   Class isAbelianGroup (G : Hask.t) {requiresSetoid : isSetoid G} : Type :=
-    { AbelianGroup_requiresGroup :> isGroup G
-    ; plu_comm :> isCommutativeBinaryOperation plu
+    { AbelianGroup_isGroup :> isGroup G
+    ; add_comm :> isCommutativeBinaryOperation add
+    }
+  .
+
+  Class Rng_sig (R : Hask.t) : Type :=
+    { mul : R -> R -> R
+    }
+  .
+
+  Class isRng (R : Hask.t) {requiresSetoid : isSetoid R} : Type :=
+    { Rng_add_isGroup :> isAbelianGroup R
+    ; Rng_mul_methods :> Rng_sig R
+    ; Rng_mul_isSemigroup :> LawsOfSemigroup R mul
+    ; Rng_requires_mul_distr_add :> isDistributiveOver mul add
+    }
+  .
+
+  Class Ring_sig (R : Hask.t) : Type :=
+    { unity : R
+    ; Ring_has_Rng_methods :> Rng_sig R
+    }
+  .
+
+  Class isRig (R : Hask.t) {requiresSetoid : isSetoid R} : Type :=
+    { Rig_add_isMonoid :> isMonoid R
+    ; Rig_mul_methods :> Ring_sig R
+    ; Rig_mul_isMonoid :> LawsOfMonoid R mul unity
+    ; Rig_requires_mul_distr_add :> isDistributiveOver mul add
     }
   .
 
